elf/ReloctablesDecode.v
@@ -6,7 +6,7 @@ Require Import encode.Hex encode.Bits.
 Import Hex Bits.
 Import ListNotations.
 Require Import SymbtableDecode ReloctablesEncode.
-Require Import RelocationTypes ReloctablesEncodeArchi.
+Require Import RelocationTypes ReloctablesEncodeArchi ReloctablesDecodeArchi.
 Set Implicit Arguments.
 
 Local Open Scope error_monad_scope.
@@ -91,93 +91,17 @@ Proof.
     destruct rt;simpl;lia.
 
 Qed.
-   
-Definition decode_relocentry (elf64: bool) (m: ZTree.t ident) (l: list byte) : res relocentry :=
-  if elf64 then
-    do (ofsbytes, l) <- take_drop 8 l;
-    do (infobytes, l) <- take_drop 8 l;
-    do (addendbytes,_) <- take_drop 8 l;
-    let ofs := decode_int ofsbytes in
-    let addend := (decode_int addendbytes) in
-    do (rt, sym) <- decode_reloc_info m infobytes;
-    OK ({| reloc_offset := ofs; reloc_type := rt; reloc_symb := sym; reloc_addend := (if zlt addend (Z.pow 2 63) then addend else addend - (Z.pow 2 64)) |})
+
+Definition acc_decode_reloctable_section (reloclen: nat) (m: ZTree.t ident) (acc: res (reloctable * list byte * nat)) (b:byte) :=
+  do acc' <- acc;
+  let '(reloctbl, reloce, len) := acc' in
+  if Nat.eq_dec len reloclen then
+    do e <- decode_relocentry decode_reloc_info Archi.ptr64 m (reloce ++ [b]);
+    OK (reloctbl ++ [e], [], 1%nat)
   else
-    do (ofsbytes, l) <- take_drop 4 l;
-    do (infobytes, l) <- take_drop 4 l;
-    let ofs := decode_int ofsbytes in
-    do (rt, sym) <- decode_reloc_info m infobytes;
-    OK ({| reloc_offset := ofs; reloc_type := rt; reloc_symb := sym; reloc_addend := 0 |}).
-
-Lemma decode_encode_relocentry: forall e m1 m2 bs (M:match_idxmap m1 m2),
-    encode_relocentry m1 e = OK bs ->
-    decode_relocentry Archi.ptr64 m2 bs = OK e.
-Proof.
-  unfold encode_relocentry,decode_relocentry.
-  intros. repeat destr_in H.
-  monadInv H11.
-  unfold encode_int64.
-  rewrite take_drop_encode_int. cbn [bind2].
-  rewrite take_drop_length_app. cbn [bind2].
-  rewrite take_drop_length. simpl. erewrite decode_encode_reloc_info;eauto.
-  simpl. destruct e. simpl in *. 
-  rewrite decode_encode_int. simpl.
-  apply andb_true_iff in Heqb. destruct Heqb.
-  rewrite Z.ltb_lt in H10.
-  rewrite Z.leb_le in H.
-  apply andb_true_iff in Heqb1. destruct Heqb1.
-  rewrite Z.ltb_lt in H12.
-  rewrite Z.leb_le in H11.
+    OK (reloctbl, reloce ++ [b], S len).
   
-  rewrite Z.mod_small;auto.
-  rewrite decode_encode_int.
-  rewrite Z.mod_small;auto.
-  unfold encode_reloc_info in EQ. repeat destr_in EQ.
-  f_equal. repeat f_equal.
-  destr.
-
-  destruct (zlt reloc_addend 0).
-  (* prove l is contradiction *)
-  apply (Z.sub_lt_mono_l _ _ (Z.pow_pos 2 64)) in l.
-  rewrite <- Z.mod_opp_l_nz in l;try lia.
-  simpl in l.
-  rewrite Z.mod_small in l;try lia.
-  unfold not. intros. apply Z.mod_opp_l_z in H13.
-  rewrite Z.mod_small in H13;try lia. lia.
-
-  rewrite Z.mod_small;try lia.
-
-  destruct (zlt reloc_addend 0).
-  apply Z.opp_inj.
-  rewrite Z.opp_sub_distr.
-  rewrite Z.add_comm. rewrite Z.add_opp_r.
-  rewrite <- Z.mod_opp_l_nz;try lia. rewrite Z.mod_small;try lia.
-
-  rewrite Z.mod_small in g;try lia.
-
-  unfold two_p. simpl. apply Z.mod_pos_bound.
-  unfold two_power_pos. simpl. lia.
-
-  rewrite encode_int_length. lia.
-
-  unfold encode_reloc_info in EQ. repeat destr_in EQ.
-  unfold encode_int64.   rewrite encode_int_length. auto.
-  
-  monadInv H11.
-
-  monadInv H11.
-  unfold encode_int32.
-  rewrite take_drop_encode_int. cbn [bind2].
-  rewrite take_drop_length. simpl. erewrite decode_encode_reloc_info;eauto.
-  simpl. destruct e. simpl in *. 
-  rewrite Z.eqb_eq in Heqb1. rewrite Heqb1.
-  rewrite decode_encode_int. simpl.
-  apply andb_true_iff in Heqb. destruct Heqb.
-  rewrite Z.ltb_lt in H10.
-  rewrite Z.leb_le in H.
-  rewrite Z.mod_small;auto.
-  unfold encode_reloc_info in EQ. repeat destr_in EQ. 
-  unfold encode_int32. rewrite encode_int_length. auto.
-  monadInv H11.
-Qed.
-
-
+Definition decode_reloctable_section (reloclen: nat) (l: list byte) (m:ZTree.t ident) :=
+  (* let reloclen := if Archi.ptr64 then 24%nat else 12%nat in *)
+  do r <- fold_left (acc_decode_reloctable_section reloclen m) l (OK ([], [], 1%nat));
+  OK (fst (fst r)).
