elf/ReloctablesEncode.v
@@ -32,13 +32,41 @@ Local Open Scope bits_scope.
 
 *)
 
+Definition encode_reloc_info (idxmap: PTree.t Z) (t:reloctype) (symb:ident)  : res (list byte) :=
+  let te := encode_reloctype t in
+  match idxmap!symb with
+  | None => Error [MSG "Relocation target symbol doesn't exist!"; CTX symb]
+  | Some idx =>
+    if Archi.ptr64 then
+      if (0 <? idx) && (idx <? Z.pow 2 32) then
+        OK (encode_int64 (idx * (Z.pow 2 32) + te))
+      else Error (msg "Overflow in encode_reloc_info")
+    else
+      if (0 <? idx) && (idx <? Z.pow 2 24) then
+        OK (encode_int32 (idx * (Z.pow 2 8) + te))
+      else Error (msg "Overflow in encode_reloc_info")
+  end.
+
+Lemma encode_reloc_info_len: forall m r id bs,
+    encode_reloc_info m r id = OK bs ->
+    length bs = if Archi.ptr64 then 8%nat else 4%nat.
+Proof.
+  unfold encode_reloc_info.
+  intros. repeat destr_in H.
+  - unfold encode_int64.
+    eapply encode_int_length.
+  - unfold encode_int32.
+    eapply encode_int_length.
+Qed.
+
+
 Section WITH_IDXMAP.
 Variable  (idxmap: PTree.t Z).
 
-
+    
 Definition acc_reloctable  acc e :=
   do acc' <- acc;
-  do bs <- encode_relocentry idxmap e;
+  do bs <- encode_relocentry idxmap encode_reloc_info e;
   OK (acc' ++ bs).
 
 Definition encode_reloctable (t: list relocentry) : res (list byte) :=
