riscV/ReloctablesEncodeArchi.v
@@ -5,6 +5,7 @@ Require Import Errors.
 Require Import RelocProg Encode RelocationTypes.
 Require Import Memdata.
 Require Import encode.Hex encode.Bits.
+Require Import LocalLib.
 Import Hex Bits.
 Import ListNotations.
 
@@ -16,27 +17,18 @@ Local Open Scope bits_scope.
 
 Section WITH_IDXMAP.
 Variable  (idxmap: PTree.t Z).
+Variable (encode_reloc_info: PTree.t Z -> reloctype -> ident -> res (list byte)).
 
-Definition encode_reloc_info (t:reloctype) (symb:ident)  : res (list byte) :=
-  let te := encode_reloctype t in
-  match idxmap!symb with
-  | None => Error [MSG "Relocation target symbol doesn't exist!"; CTX symb]
-  | Some idx =>
-    if Archi.ptr64 then
-      if (0 <? idx) && (idx <? Z.pow 2 32) then
-        OK (encode_int64 (idx * (Z.pow 2 32) + te))
-      else Error (msg "Overflow in encode_reloc_info")
-    else
-      if (0 <? idx) && (idx <? Z.pow 2 24) then
-        OK (encode_int32 (idx * (Z.pow 2 8) + te))
-      else Error (msg "Overflow in encode_reloc_info")
-  end.
+Hypothesis encode_reloc_info_len: forall m r id bs,
+    encode_reloc_info m r id = OK bs ->
+    length bs = if Archi.ptr64 then 8%nat else 4%nat.
+
 
 Definition encode_relocentry (e:relocentry) : res (list byte) :=
   let len := if Archi.ptr64 then 64 else 32 in
   if (0 <=? e.(reloc_offset)) && (e.(reloc_offset) <? Z.pow 2 len) then
     let r_offset_bytes := if Archi.ptr64 then encode_int64 (reloc_offset e)  else  encode_int32 (reloc_offset e) in    
-    do r_info_bytes <- encode_reloc_info (reloc_type e) (reloc_symb e);
+    do r_info_bytes <- encode_reloc_info idxmap (reloc_type e) (reloc_symb e);
     if Archi.ptr64 then
       if (- (Z.pow 2 63) <=? (reloc_addend e)) && ((reloc_addend e) <? (Z.pow 2 63)) then
         OK (r_offset_bytes ++ r_info_bytes ++ encode_int64 ((reloc_addend e) mod (Z.pow 2 64)))
@@ -44,7 +36,7 @@ Definition encode_relocentry (e:relocentry) : res (list byte) :=
         Error [MSG "Reloc addend overflow in 64bit mode";CTX (reloc_symb e)]
     else
       if (- (Z.pow 2 31) <=? (reloc_addend e)) && ((reloc_addend e) <? (Z.pow 2 31)) then
-        OK (r_offset_bytes ++ r_info_bytes ++ encode_int32 ((reloc_addend e) mod (Z.pow 2 31)))
+        OK (r_offset_bytes ++ r_info_bytes ++ encode_int32 ((reloc_addend e) mod (Z.pow 2 32)))
       else
         Error [MSG "Reloc addend overflow in 32bit mode";CTX (reloc_symb e)]
 
@@ -55,20 +47,25 @@ Lemma encode_relocentry_len: forall l e,
     length l = if Archi.ptr64 then 24%nat else 12%nat.
 Proof.
   unfold encode_relocentry.
-  intros. repeat destr_in H.
-  monadInv H11. unfold encode_reloc_info in EQ.
-  repeat destr_in EQ.
+  intros. repeat destr_in H.  
+  monadInv H11. 
   unfold encode_int64. repeat rewrite app_length.
-  do 3 rewrite encode_int_length. lia.
-  monadInv H11. unfold encode_reloc_info in H11.
+  exploit encode_reloc_info_len;eauto;intros INFOLEN;rewrite INFOLEN.
+  do 2 rewrite encode_int_length. lia.
+  
+  monadInv H11.
 
-  unfold encode_relocentry.
-  intros. repeat destr_in H.
-  monadInv H11. unfold encode_reloc_info in EQ.
-  repeat destr_in EQ.
-  unfold encode_int32. repeat rewrite app_length.
-  do 3 rewrite encode_int_length. lia.
+  monadInv H11. unfold encode_int32. repeat rewrite app_length.
+  exploit encode_reloc_info_len;eauto;intros INFOLEN;try rewrite INFOLEN.
+  do 2 rewrite encode_int_length. lia.
+
   monadInv H11. 
 Qed.  
 
 End WITH_IDXMAP.
+
+
+
+
+
+    
