riscV/RelocElfgenproofArchi.v
@@ -1,0 +1,199 @@
+Require Import Coqlib Maps AST lib.Integers Values.
+Require Import Events lib.Floats Memory Smallstep.
+Require Import Asm RelocProg RelocProgramBytes RelocElf Globalenvs.
+Require Import Linking RelocProgLinking RelocElfLinking Errors.
+Require Import EncDecRet RelocElfgen LocalLib RelocProgGlobalenvs.
+Require Import RelocProgSemantics RelocProgSemantics1.
+Require Import RelocProgSemantics2 RelocElfSemantics.
+Require Import SymbtableDecode ReloctablesEncode.
+Require Import RelocProgSemanticsArchi.
+Require Import ReloctablesEncodeArchi.
+Require Import RelocElfgenproof0.
+Import Hex Bits.
+Import ListNotations.
+
+Set Implicit Arguments.
+
+Local Open Scope error_monad_scope.
+Local Open Scope hex_scope.
+Local Open Scope bits_scope.
+Local Open Scope string_byte_scope.
+
+
+
+Section WITH_INSTR_SIZE.
+  Variable instr_size: instruction -> Z.
+
+Section PRESERVATION. 
+(** Transformation *)
+Variable prog: program.
+Variable tprog: elf_file.
+Hypothesis TRANSF: match_prog prog tprog.
+
+Let ge := RelocProgSemantics2.globalenv instr_size  prog.
+Let tge := globalenv instr_size  tprog.
+
+
+Lemma eval_addrmode_match_ge: forall ge1 ge2 a rs (MATCHGE: forall i ofs, RelocProgGlobalenvs.Genv.symbol_address ge1 i ofs = RelocProgGlobalenvs.Genv.symbol_address ge2 i ofs),
+    eval_addrmode ge1 a rs = eval_addrmode ge2 a rs.
+Proof.
+  unfold eval_addrmode. destruct Archi.ptr64;intros.
+  - unfold eval_addrmode64.
+    destruct a. f_equal.
+    f_equal. destr.
+    destruct p. eauto.
+  - unfold eval_addrmode32.
+    destruct a. f_equal.
+    f_equal. destr.
+    destruct p. eauto.
+Qed.
+
+Lemma exec_load_match_ge: forall sz ge1 ge2 chunk m a rs rd (MATCHGE: forall i ofs, RelocProgGlobalenvs.Genv.symbol_address ge1 i ofs = RelocProgGlobalenvs.Genv.symbol_address ge2 i ofs) ,
+          exec_load sz ge1 chunk m a rs rd = exec_load sz ge2 chunk m a rs rd.
+Proof.
+  unfold exec_load.
+  intros. erewrite eval_addrmode_match_ge.
+  eauto. auto.
+Qed.
+
+Lemma exec_store_match_ge: forall sz ge1 ge2 chunk m a rs rd l (MATCHGE: forall i ofs, RelocProgGlobalenvs.Genv.symbol_address ge1 i ofs = RelocProgGlobalenvs.Genv.symbol_address ge2 i ofs) ,
+          exec_store sz ge1 chunk m a rs rd l = exec_store sz ge2 chunk m a rs rd l.
+Proof.
+  unfold exec_store.
+  intros. erewrite eval_addrmode_match_ge.
+  eauto. auto.
+Qed.
+
+Lemma eval_builtin_arg_match_ge: forall rs sp m arg varg ge1 ge2 (MATCHGE: forall i ofs, RelocProgGlobalenvs.Genv.symbol_address ge1 i ofs = RelocProgGlobalenvs.Genv.symbol_address ge2 i ofs),
+        eval_builtin_arg preg ge1 rs sp m arg varg ->
+        eval_builtin_arg preg ge2 rs sp m arg varg.
+Proof.
+  induction 2;try constructor;auto.
+  rewrite MATCHGE in H. auto.
+  rewrite MATCHGE. constructor.
+Qed.
+
+Lemma eval_builtin_args_match_ge: forall rs sp m args vargs ge1 ge2 (MATCHGE: forall i ofs, RelocProgGlobalenvs.Genv.symbol_address ge1 i ofs = RelocProgGlobalenvs.Genv.symbol_address ge2 i ofs),
+        eval_builtin_args preg ge1 rs sp m args vargs ->
+        eval_builtin_args preg ge2 rs sp m args vargs.
+Proof.
+  induction 2.
+  - constructor.
+  - econstructor.
+    eapply eval_builtin_arg_match_ge;eauto.
+    eauto.
+Qed.
+
+Lemma step_simulation: forall st1 st2 t,
+    step instr_size ge st1 t st2 ->
+    step instr_size tge st1 t st2.
+Proof.
+  intros.
+  unfold ge,tge in *.
+  exploit gen_reloc_elf_correct;eauto.
+  unfold globalenv.
+  intros (p' & D1 & E1).
+  rewrite D1.
+  unfold RelocProgSemantics2.globalenv in *.
+  destr_in H.
+  exploit decode_prog_code_section_correct;eauto.
+  intros (p2' & D2 & E2). rewrite D2.
+
+  2: {
+    (* trivial cases *)
+  destr.
+  exploit decode_prog_code_section_correct. eapply program_equiv_sym in E1.
+  eauto. eauto.
+  intros (p2' & D2 & E2). congruence.
+
+  assert ((empty_program1 prog) = (empty_program1 p')).
+  unfold empty_program1.
+  f_equal.
+  apply pe_prog_defs;eauto.
+  apply pe_prog_main;eauto.
+  apply pe_prog_senv;eauto.
+  rewrite <- H0. auto. }
+  
+  inv H.
+  - eapply exec_step_internal;eauto.
+    + unfold RelocProgGlobalenvs.Genv.find_ext_funct in *.
+      destr. erewrite program_equiv_ext_funs1 in H1.
+      eauto. eauto.
+    + unfold RelocProgGlobalenvs.Genv.find_instr.
+      erewrite program_equiv_instr_map.
+      eauto. eapply program_equiv_sym. eauto.
+    + apply program_equiv_sym in E2.
+      destruct i;simpl in *;auto.
+      1-27: try (erewrite program_equiv_symbol_address1;eauto).
+      1-24: try (erewrite exec_load_match_ge;eauto;eapply program_equiv_symbol_address1;eauto).
+      1-12: try (erewrite exec_store_match_ge;eauto;eapply program_equiv_symbol_address1;eauto).
+      rewrite <- H3. do 3 f_equal.
+      unfold eval_addrmode32.
+      destruct a. f_equal.
+      f_equal. destr.
+      destruct p0. eapply program_equiv_symbol_address1;eauto.
+      rewrite <- H3. do 3 f_equal.
+      unfold eval_addrmode64.
+      destruct a. f_equal.
+      f_equal. destr.
+      destruct p0. eapply program_equiv_symbol_address1;eauto.
+
+  (* - eapply exec_step_builtin with (vargs:= vargs);eauto. *)
+  (*   + unfold RelocProgGlobalenvs.Genv.find_ext_funct in *. *)
+  (*     destr. erewrite program_equiv_ext_funs1 in H1. *)
+  (*     eauto. eauto. *)
+  (*   + unfold RelocProgGlobalenvs.Genv.find_instr. *)
+  (*     erewrite program_equiv_instr_map. *)
+  (*     eauto. eapply program_equiv_sym. eauto. *)
+  (*   + eapply eval_builtin_args_match_ge. *)
+  (*     eapply program_equiv_symbol_address1;eauto. *)
+  (*     eauto. *)
+  (*   + eapply external_call_symbols_preserved with (ge1:= (Genv.genv_senv (RelocProgSemantics.globalenv instr_size p))). *)
+  (*     simpl. erewrite pe_prog_senv. *)
+  (*     unfold Senv.equiv. split;eauto. *)
+  (*     auto. auto. *)
+      
+  - eapply exec_step_external;eauto.
+    + unfold RelocProgGlobalenvs.Genv.find_ext_funct in *.
+      destr. erewrite program_equiv_ext_funs1 in H1.
+      eauto. eauto.
+    + eapply external_call_symbols_preserved with (ge1:= (Genv.genv_senv (RelocProgGlobalenvs.globalenv instr_size p))).
+      simpl. erewrite pe_prog_senv.
+      unfold Senv.equiv. split;eauto.
+      auto. auto.
+Qed.
+
+
+End PRESERVATION.
+
+  
+Lemma initial_state_gen_match: forall D rs m st (p tp: RelocProg.program fundef unit instruction D),
+    program_equiv p tp ->
+    initial_state_gen instr_size (decode_program instr_size p) rs m st ->
+    exists st', initial_state_gen instr_size (decode_program instr_size tp) rs m st' /\ st = st'.
+Proof.
+  intros.
+  inv H0.
+  set (ge' := RelocProgGlobalenvs.globalenv instr_size (decode_program instr_size tp)).
+  set (rs0' :=  ((rs # PC <-
+           (Genv.symbol_address ge' (RelocProg.prog_main (decode_program instr_size tp)) Ptrofs.zero))
+          # RA <- Vnullptr) # RSP <-
+         (Vptr stk
+            (Ptrofs.sub (Ptrofs.repr (max_stacksize + align (size_chunk Mptr) 8))
+               (Ptrofs.repr (size_chunk Mptr))))).
+  
+  exists (State rs0' m2). split;auto.
+  econstructor;eauto.
+  f_equal.
+  unfold rs0,rs0'.
+  assert ((RelocProg.prog_main (decode_program instr_size p)) = (RelocProg.prog_main (decode_program instr_size tp))).
+  unfold decode_program. simpl.
+  eapply pe_prog_main;eauto.
+  rewrite H0.
+
+  unfold ge,ge'.
+  erewrite program_equiv_symbol_address;eauto.
+  eapply decode_program_equiv. auto.    
+Qed.
+
+End WITH_INSTR_SIZE.
