riscV/ReloctablesDecodeArchi.v
@@ -1,0 +1,224 @@
+Require Import Coqlib Integers AST Maps.
+Require Import Errors.
+Require Import RelocProg RelocProgramBytes Encode.
+Require Import Memdata.
+Require Import encode.Hex encode.Bits.
+Import Hex Bits.
+Import ListNotations.
+Require Import SymbtableDecode ReloctablesEncode.
+Require Import RelocationTypes ReloctablesEncodeArchi.
+Set Implicit Arguments.
+
+Local Open Scope error_monad_scope.
+Local Open Scope hex_scope.
+Local Open Scope bits_scope.
+Local Open Scope Z_scope.
+
+
+Definition decode_reloctype (z: Z) : res reloctype :=
+  match z with
+  |1  => OK R_RISCV_32     
+  |2  => OK R_RISCV_64     
+  |17 => OK R_RISCV_JAL    
+  |18 => OK R_RISCV_CALL   
+  |23 => OK R_RISCV_PCREL_HI20
+  |24 => OK R_RISCV_PCREL_LO12_I
+  |26 => OK R_RISCV_HI20   
+  |27 => OK R_RISCV_LO12_I 
+  |28 => OK R_RISCV_LO12_S
+  | _ => Error (msg "decode_reloctype: Unexpected value for symbtype")
+  end.
+
+Lemma decode_encode_reloctype rt:
+  decode_reloctype (encode_reloctype rt) = OK rt.
+Proof. destruct rt; reflexivity. Qed.
+
+Section INFO_DECODE.
+  Variable (encode_reloc_info: PTree.t Z -> reloctype -> ident -> res (list byte)).
+  Variable decode_reloc_info: ZTree.t ident -> list byte -> res (reloctype * ident).
+
+  Hypothesis encode_reloc_info_len: forall m r id bs,
+    encode_reloc_info m r id = OK bs ->
+    length bs = if Archi.ptr64 then 8%nat else 4%nat.
+  
+  Hypothesis decode_encode_reloc_info: forall bs rt symb m1 m2 (M: match_idxmap m1 m2),
+    encode_reloc_info m1 rt symb = OK bs ->
+    decode_reloc_info m2 bs = OK (rt, symb).
+
+Definition decode_relocentry (elf64: bool) (m: ZTree.t ident) (l: list byte) : res relocentry :=
+  if elf64 then
+    do (ofsbytes, l) <- take_drop 8 l;
+    do (infobytes, l) <- take_drop 8 l;
+    do (addendbytes,_) <- take_drop 8 l;
+    let ofs := decode_int ofsbytes in
+    let addend := (decode_int addendbytes) in
+    do (rt, sym) <- decode_reloc_info m infobytes;
+    OK ({| reloc_offset := ofs; reloc_type := rt; reloc_symb := sym; reloc_addend := (if zlt addend (Z.pow 2 63) then addend else addend - (Z.pow 2 64)) |})
+  else
+    do (ofsbytes, l) <- take_drop 4 l;
+    do (infobytes, l) <- take_drop 4 l;
+    do (addendbytes,_) <- take_drop 4 l;
+    let ofs := decode_int ofsbytes in
+    let addend := (decode_int addendbytes) in
+    do (rt, sym) <- decode_reloc_info m infobytes;
+    OK ({| reloc_offset := ofs; reloc_type := rt; reloc_symb := sym; reloc_addend := (if zlt addend (Z.pow 2 31) then addend else addend - (Z.pow 2 32)) |}).
+
+
+Lemma decode_encode_relocentry: forall e m1 m2 bs (M:match_idxmap m1 m2),
+    encode_relocentry m1 encode_reloc_info  e = OK bs ->
+    decode_relocentry Archi.ptr64 m2 bs = OK e.
+Proof.
+  unfold encode_relocentry,decode_relocentry.
+  intros. repeat destr_in H.
+  monadInv H11.
+  unfold encode_int64.
+  rewrite take_drop_encode_int. cbn [bind2].
+  rewrite take_drop_length_app. cbn [bind2].
+  rewrite take_drop_length. simpl. erewrite decode_encode_reloc_info;eauto.
+  simpl. destruct e. simpl in *. 
+  rewrite decode_encode_int. simpl.
+  apply andb_true_iff in Heqb. destruct Heqb.
+  rewrite Z.ltb_lt in H10.
+  rewrite Z.leb_le in H.
+  apply andb_true_iff in Heqb1. destruct Heqb1.
+  rewrite Z.ltb_lt in H12.
+  rewrite Z.leb_le in H11.
+  
+  rewrite Z.mod_small;auto.
+  rewrite decode_encode_int.
+  rewrite Z.mod_small;auto.
+  repeat f_equal.
+
+  (* Lemma two_complement_correct: forall n l, *)        
+  destr.
+
+  destruct (zlt reloc_addend 0).
+  (* prove l is contradiction *)
+  apply (Z.sub_lt_mono_l _ _ (Z.pow_pos 2 64)) in l.
+  rewrite <- Z.mod_opp_l_nz in l;try lia.
+  simpl in l.
+  rewrite Z.mod_small in l;try lia.
+  unfold not. intros. apply Z.mod_opp_l_z in H13.
+  rewrite Z.mod_small in H13;try lia. lia.
+
+  rewrite Z.mod_small;try lia.
+
+  destruct (zlt reloc_addend 0).
+  apply Z.opp_inj.
+  rewrite Z.opp_sub_distr.
+  rewrite Z.add_comm. rewrite Z.add_opp_r.
+  rewrite <- Z.mod_opp_l_nz;try lia. rewrite Z.mod_small;try lia.
+
+  rewrite Z.mod_small in g;try lia.
+
+  unfold two_p. simpl. apply Z.mod_pos_bound.
+  unfold two_power_pos. simpl. lia.
+
+  rewrite encode_int_length. lia.
+  
+  eapply encode_reloc_info_len;eauto.
+  
+  monadInv H11.
+
+  (* 32 bit mode *)
+  monadInv H11.
+  unfold encode_int32.
+  rewrite take_drop_encode_int. cbn [bind2].
+  rewrite take_drop_length_app. cbn [bind2].
+  rewrite take_drop_length. simpl. erewrite decode_encode_reloc_info;eauto.
+  simpl. destruct e. simpl in *. 
+  rewrite decode_encode_int. simpl.
+  apply andb_true_iff in Heqb. destruct Heqb.
+  rewrite Z.ltb_lt in H10.
+  rewrite Z.leb_le in H.
+  apply andb_true_iff in Heqb1. destruct Heqb1.
+  rewrite Z.ltb_lt in H12.
+  rewrite Z.leb_le in H11.
+  
+  rewrite Z.mod_small;auto.
+  rewrite decode_encode_int.
+  rewrite Z.mod_small;auto.
+  repeat f_equal.
+
+  (* Lemma two_complement_correct: forall n l, *)        
+  destr.
+
+  destruct (zlt reloc_addend 0).
+  (* prove l is contradiction *)
+
+  apply (Z.sub_lt_mono_l _ _ (Z.pow_pos 2 32)) in l.
+  rewrite <- Z.mod_opp_l_nz in l;try lia.
+  simpl in l.
+  rewrite Z.mod_small in l;try lia.
+  unfold not. intros. apply Z.mod_opp_l_z in H13.
+  rewrite Z.mod_small in H13;try lia. lia.
+
+  rewrite Z.mod_small;try lia.
+
+  destruct (zlt reloc_addend 0).
+  apply Z.opp_inj.
+  rewrite Z.opp_sub_distr.
+  rewrite Z.add_comm. rewrite Z.add_opp_r.
+  rewrite <- Z.mod_opp_l_nz;try lia. rewrite Z.mod_small;try lia.
+
+  rewrite Z.mod_small in g;try lia.
+
+  unfold two_p. simpl. apply Z.mod_pos_bound.
+  unfold two_power_pos. simpl. lia.
+
+  rewrite encode_int_length. lia.
+
+  eapply encode_reloc_info_len;eauto.
+  monadInv H11.
+Qed.
+
+
+(* (* accumulation *) *)
+(* Definition acc_decode_reloctable_section (reloclen: nat) (m: ZTree.t ident) (acc: res (reloctable * list byte * nat)) (b:byte) := *)
+(*   do acc' <- acc; *)
+(*   let '(reloctbl, reloce, len) := acc' in *)
+(*   if Nat.eq_dec len reloclen then *)
+(*     do e <- decode_relocentry Archi.ptr64 m (reloce ++ [b]); *)
+(*     OK (reloctbl ++ [e], [], 1%nat) *)
+(*   else *)
+(*     OK (reloctbl, reloce ++ [b], S len). *)
+  
+(* Definition decode_reloctable_section  (l: list byte) (m:ZTree.t ident) := *)
+(*   let reloclen := if Archi.ptr64 then 24%nat else 12%nat in *)
+(*   do r <- fold_left (acc_decode_reloctable_section reloclen m) l (OK ([], [], 1%nat)); *)
+(*   OK (fst (fst r)). *)
+
+(* Lemma decode_encode_reloctable_correct: forall n l bs m1 m2 (M: match_idxmap m1 m2), *)
+(*     let reloclen := if Archi.ptr64 then 24%nat else 12%nat in *)
+(*     length l = n -> *)
+(*     encode_reloctable m1 l = OK bs -> *)
+(*     fold_left (acc_decode_reloctable_section reloclen m2) bs (OK ([], [], 1%nat)) = OK (l, [], 1%nat). *)
+(* Proof. *)
+(*   induction n;intros l bs m1 m2 M PTR H H0. *)
+(*   rewrite length_zero_iff_nil in H. subst. *)
+(*   simpl in H0. inv H0. *)
+(*   unfold decode_reloctable_section. simpl. auto. *)
+
+(*   exploit LocalLib.length_S_inv;eauto. *)
+(*   intros (l' & a1 & A1 & B1). subst. *)
+(*   clear H. *)
+(*   unfold encode_reloctable in H0. rewrite fold_left_app in H0. *)
+(*   simpl in H0. unfold acc_reloctable in H0 at 1. *)
+(*   monadInv H0. exploit IHn;eauto. *)
+(*   intros. rewrite fold_left_app. *)
+(*   unfold PTR. *)
+(*   rewrite H. clear H EQ IHn. *)
+(*   exploit encode_relocentry_len;eauto. *)
+(*   eapply encode_reloc_info_len. *)
+(*   intros LEN. rename x0 into l. *)
+(*   clear x. *)
+(*   eapply ReloctablesDecodeArchi.decode_encode_relocentry in EQ1;eauto. *)
+(*   eapply encode_reloc_info_len. *)
+(*   destr. *)
+(*   - do 25 (destruct l as [| ?b ?] ;simpl in LEN;try congruence). *)
+(*     simpl in *. rewrite EQ1. simpl. auto. *)
+(*   - do 9 (destruct l as [| ?b ?] ;simpl in LEN;try congruence). *)
+(*     simpl in *. rewrite EQ1. simpl. auto. *)
+(* Qed. *)
+
+End INFO_DECODE.
