x86/RelocElfArchi.v
@@ -21,7 +21,7 @@ Definition machine := if ptr64 then EM_x86_64 else EM_386.
 Definition elf_flag := 0%Z.
 
 (* relocentry size *)
-Definition reloc_entry_size := if ptr64 then 24 else 8.
+Definition reloc_entry_size := if ptr64 then 24%nat else 8%nat.
 
 Definition rel_eh_type := if Archi.ptr64 then SHT_RELA else SHT_REL.
 
