x86/ReloctablesDecodeArchi.v
@@ -1,0 +1,133 @@
+Require Import Coqlib Integers AST Maps.
+Require Import Errors.
+Require Import RelocProg RelocProgramBytes Encode.
+Require Import Memdata.
+Require Import encode.Hex encode.Bits.
+Import Hex Bits.
+Import ListNotations.
+Require Import SymbtableDecode ReloctablesEncode.
+Require Import RelocationTypes ReloctablesEncodeArchi.
+Set Implicit Arguments.
+
+Local Open Scope error_monad_scope.
+Local Open Scope hex_scope.
+Local Open Scope bits_scope.
+Local Open Scope Z_scope.
+
+
+(* Decoding of relocation typem. I do not know where to place *)
+Definition decode_reloctype (z: Z) : res reloctype :=
+  match z with
+  | 0 => OK reloc_null
+  | 1 => OK reloc_abs
+  | 2 => OK reloc_rel
+  | _ => Error (msg "decode_reloctype: Unexpected value for symbtype")
+  end.
+
+Lemma decode_encode_reloctype rt:
+  decode_reloctype (encode_reloctype rt) = OK rt.
+Proof. destruct rt; reflexivity. Qed.
+
+Section INFO_DECODE.
+  Variable (encode_reloc_info: PTree.t Z -> reloctype -> ident -> res (list byte)).
+  Variable decode_reloc_info: ZTree.t ident -> list byte -> res (reloctype * ident).
+
+  Hypothesis encode_reloc_info_len: forall m r id bs,
+    encode_reloc_info m r id = OK bs ->
+    length bs = if Archi.ptr64 then 8%nat else 4%nat.
+  
+  Hypothesis decode_encode_reloc_info: forall bs rt symb m1 m2 (M: match_idxmap m1 m2),
+    encode_reloc_info m1 rt symb = OK bs ->
+    decode_reloc_info m2 bs = OK (rt, symb).
+
+   
+Definition decode_relocentry (elf64: bool) (m: ZTree.t ident) (l: list byte) : res relocentry :=
+  if elf64 then
+    do (ofsbytes, l) <- take_drop 8 l;
+    do (infobytes, l) <- take_drop 8 l;
+    do (addendbytes,_) <- take_drop 8 l;
+    let ofs := decode_int ofsbytes in
+    let addend := (decode_int addendbytes) in
+    do (rt, sym) <- decode_reloc_info m infobytes;
+    OK ({| reloc_offset := ofs; reloc_type := rt; reloc_symb := sym; reloc_addend := (if zlt addend (Z.pow 2 63) then addend else addend - (Z.pow 2 64)) |})
+  else
+    do (ofsbytes, l) <- take_drop 4 l;
+    do (infobytes, l) <- take_drop 4 l;
+    let ofs := decode_int ofsbytes in
+    do (rt, sym) <- decode_reloc_info m infobytes;
+    OK ({| reloc_offset := ofs; reloc_type := rt; reloc_symb := sym; reloc_addend := 0 |}).
+
+Lemma decode_encode_relocentry: forall e m1 m2 bs (M:match_idxmap m1 m2),
+    encode_relocentry m1 e = OK bs ->
+    decode_relocentry Archi.ptr64 m2 bs = OK e.
+Proof.
+  unfold encode_relocentry,decode_relocentry.
+  intros. repeat destr_in H.
+  monadInv H11.
+  unfold encode_int64.
+  rewrite take_drop_encode_int. cbn [bind2].
+  rewrite take_drop_length_app. cbn [bind2].
+  rewrite take_drop_length. simpl. erewrite decode_encode_reloc_info;eauto.
+  simpl. destruct e. simpl in *. 
+  rewrite decode_encode_int. simpl.
+  apply andb_true_iff in Heqb. destruct Heqb.
+  rewrite Z.ltb_lt in H10.
+  rewrite Z.leb_le in H.
+  apply andb_true_iff in Heqb1. destruct Heqb1.
+  rewrite Z.ltb_lt in H12.
+  rewrite Z.leb_le in H11.
+  
+  rewrite Z.mod_small;auto.
+  rewrite decode_encode_int.
+  rewrite Z.mod_small;auto.
+  unfold encode_reloc_info in EQ. repeat destr_in EQ.
+  f_equal. repeat f_equal.
+  destr.
+
+  destruct (zlt reloc_addend 0).
+  (* prove l is contradiction *)
+  apply (Z.sub_lt_mono_l _ _ (Z.pow_pos 2 64)) in l.
+  rewrite <- Z.mod_opp_l_nz in l;try lia.
+  simpl in l.
+  rewrite Z.mod_small in l;try lia.
+  unfold not. intros. apply Z.mod_opp_l_z in H13.
+  rewrite Z.mod_small in H13;try lia. lia.
+
+  rewrite Z.mod_small;try lia.
+
+  destruct (zlt reloc_addend 0).
+  apply Z.opp_inj.
+  rewrite Z.opp_sub_distr.
+  rewrite Z.add_comm. rewrite Z.add_opp_r.
+  rewrite <- Z.mod_opp_l_nz;try lia. rewrite Z.mod_small;try lia.
+
+  rewrite Z.mod_small in g;try lia.
+
+  unfold two_p. simpl. apply Z.mod_pos_bound.
+  unfold two_power_pos. simpl. lia.
+
+  rewrite encode_int_length. lia.
+
+  unfold encode_reloc_info in EQ. repeat destr_in EQ.
+  unfold encode_int64.   rewrite encode_int_length. auto.
+  
+  monadInv H11.
+
+  monadInv H11.
+  unfold encode_int32.
+  rewrite take_drop_encode_int. cbn [bind2].
+  rewrite take_drop_length. simpl. erewrite decode_encode_reloc_info;eauto.
+  simpl. destruct e. simpl in *. 
+  rewrite Z.eqb_eq in Heqb1. rewrite Heqb1.
+  rewrite decode_encode_int. simpl.
+  apply andb_true_iff in Heqb. destruct Heqb.
+  rewrite Z.ltb_lt in H10.
+  rewrite Z.leb_le in H.
+  rewrite Z.mod_small;auto.
+  unfold encode_reloc_info in EQ. repeat destr_in EQ. 
+  unfold encode_int32. rewrite encode_int_length. auto.
+  monadInv H11.
+Qed.
+
+
+End INFO_DECODE.
