autogen/switch.sh
@@ -1,0 +1,14 @@
+if test "$1" = "riscv"
+then
+mv EncDecRet.v EncDecRet.v.$1;
+mv VerificationCondition.v VerificationCondition.v.$1;
+mv EncDecRet.v.x86 EncDecRet.v;
+mv VerificationCondition.v.x86 VerificationCondition.v;
+else
+mv EncDecRet.v EncDecRet.v.$1;
+mv VerificationCondition.v VerificationCondition.v.$1;
+mv EncDecRet.v.riscv EncDecRet.v;
+mv VerificationCondition.v.riscv VerificationCondition.v;
+fi
+
+rm *.vo
